protocols/SimplePingProtocolAutomated.v
@@ -119,84 +119,119 @@ Section RealProtocol.
   
 End RealProtocol.
 
-Hint Unfold
-     A B PERMS__a PERMS__b
-     real_univ_start mkrU
-     ideal_univ_start mkiU : constants.
-
 Import SimulationAutomation.
-
-(* Hint Constructors *)
-(*      RSimplePing. *)
-(* Hint Extern 1 (RSimplePing (RealWorld.peel_adv _) _) => *)
-(*   simpl; simpl_real_users_context; simpl_ideal_users_context; simpl; *)
-(*    ( (eapply Start  ; solve [ eauto ]) *)
-(*    || (eapply Recd1' ; solve [ eauto ]) *)
-(*    || (eapply Sent1' ; solve [ eauto ]) ). *)
-
-Hint Extern 0 (~^* _ _) =>
- progress(unfold real_univ_start, mkrU; simpl).
-(* Hint Extern 1 (RSimplePing (RealWorld.buildUniverse _ _ _ _ _ _) _) => unfold RealWorld.buildUniverse; simpl. *)
-
-Hint Extern 0 (IdealWorld.lstep_universe _ _ _) =>
- progress(unfold ideal_univ_start, mkiU; simpl).
-
-(* Hint Extern 1 (IdealWorld.lstep_universe _ _ _) => single_step_ideal_universe; eauto 2; econstructor. *)
-Hint Extern 1 (PERMS__a $? _ = _) => unfold PERMS__a.
-Hint Extern 1 (PERMS__b $? _ = _) => unfold PERMS__b.
-
-Hint Extern 1 (istepSilent ^* _ _) =>
-unfold ideal_univ_start, mkiU; simpl;
-  repeat (ideal_single_silent_multistep A);
-  repeat (ideal_single_silent_multistep B); solve_refl.
-
 
 Import Sets.
 Module Foo <: EMPTY.
 End Foo.
 Module Import SN := SetNotations(Foo).
 
-Module PD <: ProcDef.
+Module SimplePingProtocolSecure <: AutomatedSafeProtocol.
 
   Definition t__hon := Nat.
   Definition t__adv := Unit.
+  Definition b := tt.
   Definition iu0  := ideal_univ_start.
   Definition ru0  := real_univ_start $0 [] [] 0 0 startAdv.
-End PD.
 
-Module G := Gen PD.
+  Import Gen ModelCheck Invariant Tacs SetLemmas.
 
-Import G PD ModelCheck Invariant Relations.
+  Hint Unfold t__hon t__adv b ru0 iu0 ideal_univ_start mkiU real_univ_start mkrU : core.
 
-Definition protos_ok : (RealWorld.universe t__hon t__adv * IdealWorld.universe t__hon) -> Prop :=
-  lift_fst honest_cmds_safe.
+  Lemma safe_invariant :
+    invariantFor
+      {| Initial := {(ru0, iu0)}; Step := @step t__hon t__adv  |}
+      (lift_fst honest_cmds_safe).
+  Proof.
+    eapply Invariant.invariant_weaken.
 
-Lemma g : invariantFor S protos_ok.
-Proof.
-  Hint Unfold ru0 iu0 ideal_univ_start mkiU real_univ_start mkrU.
-  eapply Invariant.invariant_weaken.
+    - apply multiStepClosure_ok; simpl.
+      gen1.
+      gen1.
+      gen1.
+      gen1.
+      gen1.
+      gen1.
+      gen1.
+      gen1.
 
-  Import Tacs SetLemmas.
+    - intros.
+      simpl in *.
+      sets_invert; unfold lift_fst;
+        split_ex; simpl in *; subst; solve_honest_actions_safe;
+          clean_map_lookups; eauto 8.
 
-  - apply multiStepClosure_ok; simpl.
-    gen1.
-    gen1.
-    gen1.
-    gen1.
-    gen1.
-    gen1.
-    gen1.
+      Unshelve.
+      all:eauto.
+  Qed.
+
+  Lemma U_good : @universe_starts_sane _ Unit b ru0.
+  Proof.
+    autounfold;
+      unfold universe_starts_sane; simpl.
+    repeat (apply conj); intros; eauto.
+    - solve_perm_merges; eauto.
+    - econstructor.
+    - unfold AdversarySafety.keys_honest, KEYS; rewrite Forall_natmap_forall; intros.
+      econstructor; simpl.
+      rewrite !findUserKeys_add_reduce, findUserKeys_empty_is_empty; eauto.
+      solve_perm_merges.
+    - unfold lameAdv; simpl; eauto.
+  Qed.
+
+  Lemma univ_ok_start : universe_ok ru0.
+  Proof.
+    autounfold; econstructor; eauto.
+  Qed.
+
+  Lemma adv_univ_ok_start : adv_universe_ok ru0.
+  Proof.
+    autounfold; unfold adv_universe_ok; eauto.
+    unfold keys_and_permissions_good.
+    pose proof (adversary_is_lame_adv_univ_ok_clauses U_good).
+
+    intuition eauto;
+      simpl in *.
+
+    - unfold KEYS in *; solve_simple_maps; eauto.
+    - rewrite Forall_natmap_forall; intros.
+      solve_simple_maps; simpl;
+        unfold permission_heap_good, KEYS, A__keys, B__keys; intros;
+          solve_simple_maps; eauto.
+
+    - unfold user_cipher_queues_ok.
+      rewrite Forall_natmap_forall; intros.
+      cases (A ==n k); cases (B ==n k);
+        subst; clean_map_lookups; simpl in *; econstructor; eauto.
+
+    - unfold honest_nonces_ok; intros.
+      unfold honest_nonce_tracking_ok.
+
+      destruct (u_id ==n A); destruct (u_id ==n B);
+        destruct (rec_u_id ==n A); destruct (rec_u_id ==n B);
+          subst; try contradiction; try discriminate; clean_map_lookups; simpl;
+            repeat (apply conj); intros; clean_map_lookups; eauto.
+
+    - unfold honest_users_only_honest_keys; intros.
+      destruct (u_id ==n A);
+        destruct (u_id ==n B);
+        subst;
+        simpl in *;
+        clean_map_lookups;
+        rewrite !findUserKeys_add_reduce, findUserKeys_empty_is_empty;
+        eauto;
+        simpl in *;
+        solve_perm_merges;
+        solve_concrete_maps;
+        solve_simple_maps;
+        eauto.
+  Qed.
+  
+  Lemma universe_starts_safe : universe_ok ru0 /\ adv_universe_ok ru0.
+  Proof.
+    repeat (simple apply conj);
+      eauto using univ_ok_start, adv_univ_ok_start.
+  Qed.
 
 
-    gen1.
-
-  - intros.
-    simpl in *.
-    sets_invert; unfold protos_ok, lift_fst;
-      split_ex; simpl in *; subst; solve_honest_actions_safe;
-        clean_map_lookups; eauto 8.
-
-    Unshelve.
-    all:eauto.
-Qed.
-    
+End SimplePingProtocolSecure.
